finished Si

Analysis/Si.thy
@@ -11,14 +11,58 @@ imports Interval_Integral
 
 begin
 
-(** Derivatives and integrals for CLT. **)
+(* copied from Distributions.borel_integral_x_exp -- only the conclusion has changed! *)
+lemma borel_integrable_x_exp:
+  "set_integrable lborel {0..} (\<lambda>x :: real. x * exp (- x))"
+proof (rule integral_monotone_convergence)
+  let ?f = "\<lambda>i x. x * exp (- x) * indicator {0::real .. i} x"
+  have "eventually (\<lambda>b::real. 0 \<le> b) at_top"
+    by (rule eventually_ge_at_top)
+  then have "eventually (\<lambda>b. 1 - (inverse (exp b) + b / exp b) = integral\<^sup>L lborel (?f b)) at_top"
+  proof eventually_elim
+   fix b :: real assume [simp]: "0 \<le> b"
+    have "(\<integral>x. (exp (-x)) * indicator {0 .. b} x \<partial>lborel) - (integral\<^sup>L lborel (?f b)) = 
+      (\<integral>x. (exp (-x) - x * exp (-x)) * indicator {0 .. b} x \<partial>lborel)"
+      by (subst integral_diff(2)[symmetric])
+         (auto intro!: borel_integrable_atLeastAtMost integral_cong split: split_indicator)
+    also have "\<dots> = b * exp (-b) - 0 * exp (- 0)"
+    proof (rule integral_FTC_atLeastAtMost)
+      fix x assume "0 \<le> x" "x \<le> b"
+      show "DERIV (\<lambda>x. x * exp (-x)) x :> exp (-x) - x * exp (-x)"
+        by (auto intro!: derivative_eq_intros)
+      show "isCont (\<lambda>x. exp (- x) - x * exp (- x)) x "
+        by (intro continuous_intros)
+    qed fact
+    also have "(\<integral>x. (exp (-x)) * indicator {0 .. b} x \<partial>lborel) = - exp (- b) - - exp (- 0)"
+      by (rule integral_FTC_atLeastAtMost) (auto intro!: derivative_eq_intros)
+    finally show "1 - (inverse (exp b) + b / exp b) = integral\<^sup>L lborel (?f b)"
+      by (auto simp: field_simps exp_minus inverse_eq_divide)
+  qed
+  then have "((\<lambda>i. integral\<^sup>L lborel (?f i)) ---> 1 - (0 + 0)) at_top"
+  proof (rule Lim_transform_eventually)
+    show "((\<lambda>i. 1 - (inverse (exp i) + i / exp i)) ---> 1 - (0 + 0 :: real)) at_top"
+      using tendsto_power_div_exp_0[of 1]
+      by (intro tendsto_intros tendsto_inverse_0_at_top exp_at_top) simp
+  qed
+  then show "(\<lambda>i. integral\<^sup>L lborel (?f i)) ----> 1"
+    by (intro filterlim_compose[OF _ filterlim_real_sequentially]) simp
+  show "AE x in lborel. mono (\<lambda>n::nat. x * exp (- x) * indicator {0..real n} x)"
+    by (auto simp: mono_def mult_le_0_iff zero_le_mult_iff split: split_indicator)
+  show "\<And>i::nat. integrable lborel (\<lambda>x. x * exp (- x) * indicator {0..real i} x)"
+    by (rule borel_integrable_atLeastAtMost) auto
+  show "AE x in lborel. (\<lambda>i. x * exp (- x) * indicator {0..real i} x) ----> x * exp (- x) * indicator {0..} x"
+    apply (intro AE_I2 Lim_eventually )
+    apply (rule_tac c="natfloor x + 1" in eventually_sequentiallyI)
+    apply (auto simp add: not_le dest!: ge_natfloor_plus_one_imp_gt[simplified] split: split_indicator)
+    done
+qed (auto intro!: borel_measurable_times borel_measurable_exp)
 
 lemma integral_expneg_alpha_atLeast0:
   fixes u :: real
   assumes pos: "0 < u"
   shows
-    "set_integrable lborel (einterval 0 \<infinity>) (\<lambda>x. exp (-x * u))" 
-    "LBINT x=0..\<infinity>. exp (-x * u) = 1/u"
+    "set_integrable lborel {0<..} (\<lambda>x. exp (-(x * u)))" 
+    "LBINT x=0..\<infinity>. exp (-(x * u)) = 1/u"
 proof -
   have 1: "0 < u \<Longrightarrow> (((\<lambda>x. - (exp (- (x * u)) / u)) \<circ> real) ---> - (1 / u)) (at_right (0::ereal))"
     apply (subgoal_tac "(((\<lambda>x. - (exp (- (x * u)) / u)) \<circ> real) ---> - (1 / u)) (at 0)")
@@ -45,14 +89,16 @@ proof -
     apply (rule filterlim_tendsto_pos_mult_at_top [OF _ pos])
     apply auto
     by (rule filterlim_ident)
-  show "LBINT x=0..\<infinity>. exp (-x * u) = 1/u"
+  show "LBINT x=0..\<infinity>. exp (-(x * u)) = 1/u"
     apply (subst interval_integral_FTC_nonneg[of _ _ "\<lambda>x. -(1/u) * exp (-x * u)" _ "-(1/u)" 0])
     using pos apply (auto intro!: derivative_eq_intros)
     by (erule 1, erule 2)
-  show "set_integrable lborel (einterval 0 \<infinity>) (\<lambda>x. exp (-x * u))"
+  have "set_integrable lborel (einterval 0 \<infinity>) (\<lambda>x. exp (-x * u))"
     apply (subst interval_integral_FTC_nonneg[of _ _ "\<lambda>x. -(1/u) * exp (-x * u)" _ "-(1/u)" 0])
     using pos apply (auto intro!: derivative_eq_intros)
     by (erule 1, erule 2)
+  thus "set_integrable lborel {0<..} (\<lambda>x. exp (-(x * u)))"
+    by (auto simp add: zero_ereal_def)
 qed
 
 lemma Collect_eq_Icc: "{r. t \<le> r \<and> r \<le> b} = {t .. b}"
@@ -61,8 +107,8 @@ lemma Collect_eq_Icc: "{r. t \<le> r \<and> r \<le> b} = {t .. b}"
 (* From Billingsley section 18. *)
 lemma ex_18_4_1:
   assumes "t \<ge> 0"
-  shows "LBINT x=0..t. exp (-u * x) * sin x = (1/(1+u^2)) *
-  (1 - exp (-u * t) * (u * sin t + cos t))"
+  shows "LBINT x=0..t. exp (-(u * x)) * sin x = (1/(1+u^2)) *
+  (1 - exp (-(u * t)) * (u * sin t + cos t))"
 
   apply (subst zero_ereal_def)
   apply (subst interval_integral_FTC_finite 
@@ -174,10 +220,78 @@ proof -
     by (rule filterlim_tan_at_right)
 qed
 
+(* a slight modification of the preceding one *)
+lemma Billingsley_ex_17_5': 
+  shows "set_integrable lborel (einterval 0 \<infinity>) (\<lambda>x. inverse (1 + x^2))"
+    "LBINT x=0..\<infinity>. inverse (1 + x^2) = pi / 2"
+proof -
+  have "(tan ---> tan 0) (at 0)"
+    by (rule tendsto_tan, auto intro: tendsto_ident_at)
+  hence [intro]: "(tan ---> 0) (at_right 0)"
+    by (rule filterlim_mono, auto simp add: at_eq_sup_left_right)
+  have 1: "\<And>x. 0 < x \<Longrightarrow> x * 2 < pi \<Longrightarrow> (tan has_real_derivative 1 + (tan x)\<^sup>2) (at x)"
+    apply (subst tan_sec)
+    apply (subgoal_tac "cos x > 0", force)
+    apply (rule cos_gt_zero_pi, auto)
+    apply (subst nonzero_power_inverse [symmetric])
+    apply (subgoal_tac "cos x > 0", force)
+    apply (rule cos_gt_zero_pi, auto)
+    apply (rule DERIV_tan)
+    apply (subgoal_tac "cos x > 0", force)
+    by (rule cos_gt_zero_pi, auto)
+  have 2: "\<And>x. 0 < x \<Longrightarrow> x * 2 < pi \<Longrightarrow> isCont (\<lambda>x. 1 + (tan x)\<^sup>2) x"
+    apply (rule isCont_add, force)
+    apply (subst power2_eq_square)
+    apply (rule isCont_mult)
+    apply (rule isCont_tan)
+    apply (subgoal_tac "cos x > 0", force)
+    apply (rule cos_gt_zero_pi, auto)
+    apply (rule isCont_tan)
+    apply (subgoal_tac "cos x > 0", force)
+    by (rule cos_gt_zero_pi, auto)
+  show "LBINT x=0..\<infinity>. inverse (1 + x^2) = pi / 2"
+    apply (subst interval_integral_substitution_nonneg[of "0" "pi/2" tan "\<lambda>x. 1 + (tan x)^2"])
+    apply (auto intro: derivative_eq_intros simp add: ereal_tendsto_simps filterlim_tan_at_left
+      zero_ereal_def)
+    apply (erule (1) 1)
+    by (erule (1) 2)
+  show "set_integrable lborel (einterval 0 \<infinity>) (\<lambda>x. inverse (1 + x^2))"
+    apply (subst interval_integral_substitution_nonneg[of "0" "pi/2" tan "\<lambda>x. 1 + (tan x)^2"])
+    apply (auto intro: derivative_eq_intros simp add: ereal_tendsto_simps filterlim_tan_at_left
+      zero_ereal_def)
+    apply (erule (1) 1)
+    by (erule (1) 2)
+qed
+
+abbreviation sinc :: "real \<Rightarrow> real" where
+  "sinc \<equiv> (\<lambda>x. if x = 0 then 1 else sin x / x)"
+
+lemma sinc_at_0: "((\<lambda>x. sin x / x) ---> 1) (at 0)"
+using DERIV_sin [of 0] by (auto simp add: has_field_derivative_def field_has_derivative_at)
+
+lemma isCont_sinc: "isCont sinc x"
+  apply (case_tac "x = 0", auto)
+  apply (simp add: isCont_def)
+  apply (subst LIM_equal [where g = "\<lambda>x. sin x / x"], auto intro: sinc_at_0)
+  apply (rule continuous_transform_at [where d = "abs x" and f = "\<lambda>x. sin x / x"])
+  by (auto simp add: dist_real_def)
+
+lemma sinc_AE: "AE x in lborel. sin x / x = sinc x"
+  by (rule AE_I [where N = "{0}"], auto)
+
 definition Si :: "real \<Rightarrow> real" where "Si t \<equiv> LBINT x=0..t. sin x / x"
+
+lemma Si_alt_def : "Si t = LBINT x=0..t. sinc x"
+  apply (case_tac "0 \<le> t")
+  unfolding Si_def apply (rule interval_lebesgue_integral_cong_AE, auto)
+  apply (rule AE_I' [where N = "{0}"], auto)
+  apply (subst (1 2) interval_integral_endpoints_reverse, simp)
+  apply (rule interval_lebesgue_integral_cong_AE, auto)
+by (rule AE_I' [where N = "{0}"], auto)
 
 (** Add to main Lebesgue integration library; does not require integrability as hypothesis, which in
 my experience greatly increases usability. **)
+(** JDA: this is probably not needed if we keep track of integrability hypotheses *)
 lemma positive_integral_eq_integral_measurable:
   assumes f: "f \<in> borel_measurable M" and I: "integral\<^sup>L M f \<noteq> 0"
   assumes nonneg: "AE x in M. 0 \<le> f x" 
@@ -196,6 +310,8 @@ proof -
     using I ereal_eq_0 by metis
 qed
 
+(* This is really needed in the library -- it is a canonical way to show that something
+   is integrable wrt a product measure. *)
 lemma (in pair_sigma_finite) Fubini_integrable_nonneg:
   assumes f[measurable]: "f \<in> borel_measurable (M1 \<Otimes>\<^sub>M M2)"
     and nonneg [simp]: "\<And>p. f p \<ge> 0"
@@ -222,76 +338,9 @@ lemma  interval_Fubini_integral:
   fixes a b c d :: ereal
   assumes ab: "a < b" and dc: "c < d" (* Interesting: cd is a reserved word. *)
     and M1: "sigma_finite_measure M1" and M2: "sigma_finite_measure M2"
-    and f: "integrable (M1 \<Otimes>\<^sub>M M2) f"
+    and f: "integrable (M1 \<Otimes>\<^sub>M M2) f" (* add indicators *)
   shows "LINT y=a..b|M2. (LINT x=c..d|M1. f (x, y)) = LINT x=c..d|M1. (LINT y=a..b|M2. f (x, y))"
-apply unfold_locales unfolding interval_lebesgue_integral_def einterval_def
-apply (auto intro: assms(1) assms(2) less_imp_le)
-(* Need to determine how to deal with the indicator functions. *)
-using pair_sigma_finite.Fubini_integral[of M1 M2] assms unfolding pair_sigma_finite_def sorry
 *)
-  
-lemma Si_at_top_lemma1:
-  fixes t :: real
-  assumes "t \<ge> 0"
-  shows "Si t = pi / 2 - (LBINT u=0..\<infinity>. inverse (1 + u^2) * exp (-u * t) * (u * sin t + cos t))"
-proof -
-  have 179: "LBINT x=0..\<infinity>. inverse (1 + x^2) = pi / 2"
-  proof -
-    have "LBINT x=-\<infinity>..\<infinity>. inverse (1 + x^2) = (LBINT x=-\<infinity>..0. inverse (1 + x^2)) +
-                                               (LBINT x=0..\<infinity>. inverse (1 + x^2))"
-      apply (subst interval_integral_sum[of "-\<infinity>" "\<infinity>" 0 "\<lambda>x. inverse (1 + x^2)",symmetric], auto)
-      apply (unfold interval_lebesgue_integrable_def einterval_def integrable_def, auto)
-      apply (subst power2_eq_square, auto)
-      apply (subst (asm) positive_integral_eq_integral_measurable)
-      apply (subst power2_eq_square, auto)
-      using Billingsley_ex_17_5 (2) unfolding interval_lebesgue_integral_def einterval_def max_def min_def
-      apply auto
-      apply (subst (asm) positive_integral_max_0[symmetric])
-      apply (subst (asm) power2_eq_square)
-    proof -
-      have *: "\<And>x. max 0 (ereal (- inverse (1 + x * x))) = 0"
-        by (metis comm_semiring_1_class.normalizing_semiring_rules(4) ereal_max_0
-            inverse_minus_eq inverse_nonpositive_iff_nonpositive le_add_same_cancel1 max.boundedE
-            max.order_iff neg_le_0_iff_le zero_ereal_def zero_le_double_add_iff_zero_le_single_add
-            zero_le_square)
-        assume "\<integral>\<^sup>+ x. max 0 (ereal (- inverse (1 + x * x))) \<partial>lborel = \<infinity>"
-        thus False by (subst (asm) *) auto
-    qed
-    moreover have "(LBINT x=-\<infinity>..0. inverse (1 + x^2)) = (LBINT x=0..\<infinity>. inverse (1 + x^2))"
-      unfolding interval_lebesgue_integral_def einterval_def apply auto
-      apply (subst power2_eq_square)+
-      apply (subst lebesgue_integral_real_affine[of "-1" "\<lambda>x. inverse (1 + x * x) * indicator {x. 0 < x} x" 0])
-      by (auto simp add: indicator_def)
-    ultimately show ?thesis using Billingsley_ex_17_5 by simp
-  qed
-  have "AE x \<in> {0..} in lborel. LBINT u=0..\<infinity>. exp (-u * x) = 1/x"
-    apply (rule AE_I[where N = "{0}"], auto)
-    apply (subst (asm) minus_mult_left)
-    using integral_expneg_alpha_atLeast0 using less_eq_real_def by metis
-  hence "Si t = LBINT x=0..t. sin x * (LBINT u=0..\<infinity>. exp (-u * x))" unfolding Si_def
-    apply (subst field_divide_inverse)
-    apply (subst inverse_eq_divide)
-    apply (rule interval_integral_cong_AE)
-    apply (rule AE_I' [where N = "{0}"], auto)
-    apply (subst (asm) (2) mult_minus_left [symmetric])
-    apply (subst (asm) integral_expneg_alpha_atLeast0)
-    unfolding einterval_def apply auto
-    apply (subst (asm) min_absorb1)
-    using assms by auto
-  also have  "... = LBINT x=0..t. (LBINT u=0..\<infinity>. sin x * exp (-u * x))"
-    apply (rule interval_lebesgue_integral_cong, auto simp add: assms einterval_def)
-    apply (subst interval_lebesgue_integral_cmult(2))
-    apply (simp add: interval_lebesgue_integrable_def)
-    apply (subst mult_minus_left [symmetric])
-    by (rule integral_expneg_alpha_atLeast0, auto)
-  also have "... = LBINT u=0..\<infinity>. (LBINT x=0..t. sin x * exp (-u * x))"
-    using interval_Fubini_integral[of 0 \<infinity> 0 "ereal t" lborel lborel "\<lambda>(u, x). sin x * exp (- (u * x))",symmetric]
-    apply auto sorry
-  also have "... = (LBINT u=0..\<infinity>. inverse (1 + u^2)) - (LBINT u=0..\<infinity>. inverse (1 + u^2) *
-    exp (-u * t) * (u * sin t + cos t))" sorry
-  finally show "Si t = pi / 2 - (LBINT u=0..\<infinity>. inverse (1 + u^2) * exp (-u * t) *
-    (u * sin t + cos t))" using 179 by simp
-qed
 
 
 (* This is useful to apply the dominated convergence theorem. Are there better ways of
@@ -309,40 +358,592 @@ lemma tendsto_at_top_imp_sequentially:
   apply (rule *, auto)
   by (erule filterlim_inverse_at_top, auto)
 
+lemma tendsto_at_top_imp_sequentially':
+  fixes f :: "real => real"
+  assumes *: "\<And>Y. (\<forall>n. Y n \<ge> B) \<Longrightarrow> filterlim Y at_top sequentially \<Longrightarrow> (\<lambda>n. f (Y n)) ----> a"
+  shows "((f ---> a) at_top)"
+proof (rule tendsto_at_top_imp_sequentially)
+  fix Y :: "nat \<Rightarrow> real"
+  assume 2: "filterlim Y at_top sequentially"
+  hence 3: "eventually (\<lambda>n. Y n \<ge> B) sequentially" by (simp add: filterlim_at_top)
+  hence "\<exists>N. \<forall>n \<ge> N. Y n \<ge> B" by (simp add: eventually_sequentially)
+  then obtain N where N: "\<forall>n \<ge> N. Y n \<ge> B" ..
+  let ?Y' = "\<lambda>n. Y (n + N)"
+  from N have 4: "(\<forall>n. ?Y' n \<ge> B)" by auto
+  from 2 have 5: "filterlim ?Y' at_top sequentially" apply (simp add: filterlim_at_top)
+    by (auto intro!: sequentially_offset)
+  have "(\<lambda>n. f (?Y' n)) ----> a" by (rule * [OF 4 5])
+  thus "(\<lambda>n. f (Y n)) ----> a" by (rule LIMSEQ_offset)
+qed
+
 lemma interval_integral_to_infinity_eq: "(LINT x=ereal a..\<infinity> | M. f x) = (LINT x : {a<..} | M. f x)"
   unfolding interval_lebesgue_integral_def by auto
 
-lemma Si_at_top_lemma2:
-  fixes t :: real
-  assumes "t \<ge> 0"
-  shows "((\<lambda>t. LBINT u=0..\<infinity>. inverse (1 + u^2) * exp (-u * t) * (u * sin t + cos t)) ---> 0) (at_top)"
-proof -
-  have 1: "\<And>t. set_integrable lborel {0<..} (\<lambda>x. inverse (1 + x\<^sup>2) * exp (- (x * t)) *
-              (x * sin t + cos t))"
-    sorry
-  have 2: "\<And>x t. \<bar>inverse (1 + x\<^sup>2) * exp (- x * t) *
-                        (x * sin t + cos t) *
-                        indicator {0<..} x\<bar>
-                       \<le> inverse (1 + x^2) * indicator {0<..} x"
-    sorry
+lemma interval_integrable_to_infinity_eq: "(interval_lebesgue_integrable M a \<infinity> f) = 
+  (set_integrable M {a<..} f)"
+  unfolding interval_lebesgue_integrable_def by auto
 
-  show ?thesis 
-    apply (rule tendsto_at_top_imp_sequentially)
+lemma at_right_le_at: "(at_right (x::'a::linorder_topology)) \<le> (at x)" 
+  by (simp add: at_eq_sup_left_right)
+
+(* can this be generalized? *)
+lemma tendsto_divide_constant: "(f ---> (l :: real)) F \<Longrightarrow> ((\<lambda>x. f x / t) ---> (l / t)) F"
+  apply (auto simp add: field_divide_inverse)
+  by (auto intro: tendsto_intros)
+
+lemma set_integrable_abs_iff:
+    "set_borel_measurable M A f \<Longrightarrow>
+    set_integrable M A (\<lambda>x. \<bar>f x\<bar>) = set_integrable M A f" 
+using integrable_abs_iff [of "\<lambda>x. f x * indicator A x" M, symmetric] by (simp add: abs_mult)
+
+lemma set_integrable_abs_iff':
+    "f \<in> borel_measurable M \<Longrightarrow> A \<in> sets M \<Longrightarrow> 
+    set_integrable M A (\<lambda>x. \<bar>f x\<bar>) = set_integrable M A f"
+by (subst set_integrable_abs_iff, auto)
+
+lemma interval_integrable_abs_iff:
+    "f \<in> borel_measurable lborel \<Longrightarrow>
+    interval_lebesgue_integrable lborel a b (\<lambda>x. \<bar>f x\<bar>) = interval_lebesgue_integrable lborel a b f"
+unfolding interval_lebesgue_integrable_def
+  by (auto simp add: set_integrable_abs_iff')
+
+(* TODO: could restrict to the set *)
+lemma set_integrable_cong_AE:
+    "f \<in> borel_measurable M \<Longrightarrow> g \<in> borel_measurable M \<Longrightarrow>
+    AE x in M. f x = g x \<Longrightarrow> A \<in> sets M \<Longrightarrow> 
+    set_integrable M A f = set_integrable M A g"
+  unfolding interval_lebesgue_integrable_def by (rule integrable_cong_AE, auto)
+
+(* TODO: could restrict to the interval *)
+lemma interval_lebesgue_integrable_cong_AE:
+    "f \<in> borel_measurable lborel \<Longrightarrow> g \<in> borel_measurable lborel \<Longrightarrow>
+    AE x in lborel. f x = g x \<Longrightarrow>
+    interval_lebesgue_integrable lborel a b f = interval_lebesgue_integrable lborel a b g"
+  unfolding interval_lebesgue_integrable_def 
+  apply (case_tac "a \<le> b", simp_all)
+  apply (rule set_integrable_cong_AE)
+  apply auto [4]
+  apply (rule set_integrable_cong_AE)
+by auto
+
+lemma Si_at_top_lemma:
+  shows "\<And>t. t \<ge> 0 \<Longrightarrow> interval_lebesgue_integrable lborel 0 \<infinity>
+     (\<lambda>x. exp (- (x * t)) * (x * sin t + cos t) / (1 + x\<^sup>2))"
+  and
+    "((\<lambda>t. (LBINT x=0..\<infinity>. exp (-(x * t)) * (x * sin t + cos t) / (1 + x^2))) ---> 0) at_top"
+proof -
+  have int1: "set_integrable lborel {0<..} (\<lambda>x. exp (- x) * \<bar>x\<bar>)"
+    apply (subst integrable_cong_AE)
+    prefer 4
+    apply (rule borel_integrable_x_exp)
+    apply auto
+    apply (rule AE_I [where N = "{0}"])
+    by (auto split: split_indicator)
+  have int2: "set_integrable lborel {0<..} (\<lambda>x. exp (- x))"
+    using integral_expneg_alpha_atLeast0 [of 1] by auto
+  {
+    fix t x :: real
+    assume "t > 0"
+    hence "exp (- x) * \<bar>x * sin t / t + cos t\<bar> * indicator {0<..} x /
+           ((1 + (x / t)\<^sup>2) * t) \<le> exp (- x) * (abs x / t + 1) / t * indicator {0<..} x"
+      apply (simp add: field_simps split: split_indicator)
+      apply (subst pos_divide_le_eq)
+      apply (rule add_pos_nonneg)
+      apply (auto simp add: field_simps)
+      apply (rule order_trans)
+      apply (rule mult_left_mono)+
+      apply (rule order_trans)
+      apply (rule abs_triangle_ineq)
+      apply (rule add_mono, subst abs_mult)
+      apply (rule mult_left_mono, rule abs_cos_le_one)
+      prefer 2
+      apply (subst abs_mult, rule mult_left_mono, rule abs_sin_le_one)
+      by (auto simp add: field_simps)
+  } note aux1 = this
+  {
+    fix t :: real
+    assume "t > 0"
+    have "set_integrable lborel {0<..} (\<lambda>x. exp (- x) * (\<bar>x\<bar> / t + 1) / t)"
+      apply (subst field_divide_inverse)+
+      apply (subst (3) mult_commute)
+      apply (rule set_integral_cmult)
+      apply (subst distrib_left)
+      apply (rule set_integral_add)
+      apply (subst mult_assoc [symmetric])
+      apply (subst (2) mult_commute)
+      apply (rule set_integral_cmult)
+      apply (rule int1)
+      apply simp
+      by (rule int2)
+  } note aux2 = this
+  { 
+    fix t :: real
+    assume "t \<ge> 0"
+    hence "integrable lborel (\<lambda>x. exp (- x) * \<bar>x * sin t / t + cos t\<bar> *
+           indicator {0<..} x / ((1 + (x / t)\<^sup>2) * t))"
+      apply (case_tac "t = 0")
+      apply simp
+      apply (rule integrable_bound)
+      prefer 2
+      apply (subst abs_of_nonneg, force)
+      apply (rule AE_I2 [OF aux1])
+      apply force
+      apply (rule aux2)
+      apply auto
+      apply measurable
+      apply auto
+      apply (subst greaterThan_def [symmetric], auto)
+      apply (subst mult_commute, subst power2_eq_square)
+      by measurable
+  } note aux3 = this      
+  {
+    fix t :: real
+    assume [arith]: "t \<ge> 0"
+    have 1: "\<And>x. 0 < ereal x \<Longrightarrow> ereal x < \<infinity> \<Longrightarrow> ((\<lambda>x. x / t) has_real_derivative (1 /t)) (at x)"
+      apply (case_tac "t = 0", auto)
+      by (auto intro!: derivative_eq_intros tendsto_divide_constant)
+    have "interval_lebesgue_integrable lborel 0 \<infinity>
+       (\<lambda>x. exp (- (x * t)) * abs (x * sin t + cos t) / (1 + x\<^sup>2))"
+      unfolding interval_lebesgue_integrable_def
+      apply (subst if_P, force)
+      apply (case_tac "t = 0")
+      using Billingsley_ex_17_5' (1) apply (simp add: field_simps)
+      apply (subst zero_ereal_def)
+      apply (rule interval_integral_substitution_nonneg [of "ereal 0" \<infinity>, OF _ 1])
+      apply (auto simp add: ereal_tendsto_simps)
+      apply (rule tendsto_mono [OF at_right_le_at])
+      apply (subgoal_tac "0 = 0 / t")
+      apply (erule ssubst) back back
+      apply (rule tendsto_divide_constant, auto intro!: tendsto_ident_at)
+      apply (subst field_divide_inverse, subst mult_commute)
+      apply (rule filterlim_tendsto_pos_mult_at_top)
+      apply (rule tendsto_const, auto intro!: filterlim_ident)
+      by (rule aux3, simp)
+  } note aux4 = this
+  {
+    fix t :: real
+    assume "t \<ge> 0"
+    hence *: "(\<lambda>x. \<bar>exp (- (x * t)) * (x * sin t + cos t) / (1 + x\<^sup>2)\<bar>) = 
+           (\<lambda>x. exp (- (x * t)) * abs (x * sin t + cos t) / (1 + x\<^sup>2))"
+      by (intro ext, auto simp add: abs_mult)
+    show "interval_lebesgue_integrable lborel 0 \<infinity>
+       (\<lambda>x. exp (- (x * t)) * (x * sin t + cos t) / (1 + x\<^sup>2))"
+      apply (subst interval_integrable_abs_iff [symmetric])
+      apply (subst power2_eq_square)
+      apply measurable  (* measurable should work with squaring, etc. *)
+      by (subst *, rule aux4 [OF `t \<ge> 0`])
+  } note aux5 = this
+  {
+    fix t x :: real
+    have "\<bar>exp (- (x * t)) * (x * sin t + cos t) / (1 + x\<^sup>2) * indicator {0<..} x\<bar> = 
+       exp (- (x * t)) * abs (x * sin t + cos t) / (1 + x\<^sup>2) * indicator {0<..} x"
+      by (auto simp add: abs_mult)
+    also have "\<dots> \<le> exp (- (x * t)) * (x + 1) / 1 * indicator {0<..} x"
+      apply (case_tac "x > 0")
+      prefer 2 apply force
+      apply (rule mult_right_mono)
+      apply (rule frac_le, force)
+      apply (rule mult_left_mono)
+      apply (rule order_trans [OF abs_triangle_ineq])
+      apply (rule add_mono)
+      by (auto simp add: abs_mult)
+    also have "\<dots> = (exp (- (x * t)) * x + exp (- (x* t))) * indicator {0<..} x" 
+      by (simp add: field_simps)
+    finally have "\<bar>exp (- (x * t)) * (x * sin t + cos t) / (1 + x\<^sup>2) * indicator {0<..} x\<bar> \<le>
+       (exp (- (x * t)) * x + exp (- (x * t))) * indicator {0<..} x" .
+  } note aux6 = this
+  {
+    fix t :: real
+    assume "t \<ge> 1"
+    have "AE x in lborel. \<bar>exp (- (x * t)) * (x * sin t + cos t) / (1 + x\<^sup>2) * indicator {0<..} x\<bar>
+         \<le> (exp (- x) * x + exp (- x)) * indicator {0<..} x"
+       apply (rule AE_I2)
+       apply (case_tac "x > 0")
+       apply (rule order_trans [OF aux6])
+       apply (rule mult_right_mono)
+       apply (rule add_mono)
+       apply (rule mult_right_mono)
+       using `t \<ge> 1` by (auto simp add: exp_le_cancel_iff)
+  } note aux7 = this
+  { 
+     fix Y :: "nat \<Rightarrow> real"
+     assume Ypos: "\<forall>n. 1 \<le> Y n" and
+       Y: "filterlim Y at_top sequentially"
+     {
+       fix x :: real 
+       assume "x > 0"
+       have "(\<lambda>n. exp (- (x * Y n))) ----> 0"
+         apply (rule filterlim_compose [OF exp_at_bot])
+         apply (subst filterlim_uminus_at_top [symmetric])
+         apply (rule filterlim_tendsto_pos_mult_at_top [OF _ `x > 0` Y])
+         by (rule tendsto_const)
+     } note aux8a = this
+     {
+       fix x :: real 
+       assume "x > 0"
+       hence "(\<lambda>n. exp (- (x * Y n)) * x) = (\<lambda>n. inverse (Y n) * ((x * Y n)^1 / exp (x * Y n)))"
+         apply (intro ext)
+         apply (auto simp add: field_simps exp_minus)
+         using Ypos by (metis not_one_le_zero)  (* other automated tools should get this! *)
+       hence "(\<lambda>n. exp (- (x * Y n)) * x) ----> 0"
+         apply (elim ssubst)
+         apply (rule tendsto_mult_zero)
+         apply (rule tendsto_inverse_0_at_top [OF Y])
+         apply (rule filterlim_compose [OF tendsto_power_div_exp_0])
+         apply (rule filterlim_tendsto_pos_mult_at_top [OF _ `x > 0` Y])
+         by (rule tendsto_const)
+     } note aux8b = this
+     have "AE x in lborel. (\<lambda>n. exp (- (x * Y n)) * (x * sin (Y n) + cos (Y n)) / (1 + x\<^sup>2) *
+         indicator {0<..} x) ----> 0"
+       apply (rule AE_I2)
+       apply (rule Lim_null_comparison)
+       apply (rule always_eventually, rule allI, subst real_norm_def)
+       apply (rule aux6)
+       apply (auto split: split_indicator)
+       by (rule tendsto_add_zero [OF aux8b aux8a])
+     hence "AE x in lborel. (\<lambda>n. exp (- (x * Y n)) * (x * sin (Y n) + cos (Y n)) / (1 + x\<^sup>2) *
+          indicator {0<..} x) ----> 0 * indicator {0<..} x"
+       by simp
+  } note aux8 = this
+  have aux9: "set_integrable lborel {0<..} (\<lambda>x. exp (- x) * x + exp (- x))"
+    apply (rule set_integral_add)
+    apply (subst mult_commute)
+    apply (subst integrable_cong_AE)
+    prefer 4 apply (rule borel_integrable_x_exp)
+    apply auto [2]
+    apply (rule AE_I' [where N = "{0}"])
+    apply auto [2]
+    apply (case_tac "x > 0", force, force)
+    using integral_expneg_alpha_atLeast0 [of 1] by simp
+  show "((\<lambda>t. (LBINT x=0..\<infinity>. exp (-(x * t)) * (x * sin t + cos t) / (1 + x^2))) ---> 0) at_top"
+    apply (rule tendsto_at_top_imp_sequentially' [of 1])
     apply (subst zero_ereal_def)
     apply (subst interval_integral_to_infinity_eq)
     apply (subgoal_tac "0 = (LBINT x:{0<..}. 0)")
     apply (erule ssubst) back
-    apply (rule integral_dominated_convergence) 
-    apply (auto intro: 1)
-    sorry 
+    apply (rule integral_dominated_convergence [OF _ aux7 aux9 aux8])
+    apply (subst interval_integrable_to_infinity_eq [symmetric])
+    apply (subst zero_ereal_def [symmetric], rule aux5)
+    apply (drule_tac x = n in spec, arith)
+    by auto
 qed
 
-lemma Si_at_top: "(Si ---> pi / 2) at_top"
-  sorry
+lemma Si_at_top:
+  shows "(Si ---> pi / 2) at_top"
+proof -
+  interpret P : pair_sigma_finite lborel lborel by unfold_locales
+{
+  fix t :: real
+  assume "t \<ge> 0"
+  { 
+    fix x 
+    have *: "(\<lambda>y. \<bar>sin x\<bar> * exp (- (y * x)) * indicator {0<..} y * indicator {0<..<t} x) =
+        (\<lambda>y. (\<bar>sin x\<bar> * indicator {0<..<t} x) * exp (- (y * x)) * indicator {0<..} y)"
+      by (simp add: field_simps)
+    have "integrable lborel (\<lambda>y. \<bar>sin x\<bar> * exp (- (y * x)) * indicator {0<..} y *
+        indicator {0<..<t} x)"
+      apply (case_tac "x > 0", auto)
+      apply (subst *)
+      by (rule set_integral_cmult, erule integral_expneg_alpha_atLeast0)
+  } note 1 = this
+  have "(\<lambda>x. LBINT y. \<bar>sin x\<bar> * exp (- (y * x)) * indicator {0<..} y * indicator {0<..<t} x) =
+        (\<lambda>x. \<bar>sin x\<bar> * indicator {0<..<t} x * (LBINT y.  exp (- (y * x)) * indicator {0<..} y))"
+    apply (rule ext)
+    apply (case_tac "x > 0", auto)
+    apply (subst set_integral_cmult (2) [symmetric])
+    apply (erule integral_expneg_alpha_atLeast0)
+    by (simp add: field_simps)
+  also have "\<dots> = (\<lambda>x. \<bar>sin x\<bar> * indicator {0<..<t} x * (1 / x))"
+    apply (rule ext)
+    apply (case_tac "x > 0")
+    apply (subst integral_expneg_alpha_atLeast0 (2) [symmetric])
+    by (auto simp add: interval_lebesgue_integral_def zero_ereal_def)
+  also have "\<dots> = (\<lambda>x. \<bar>sin x\<bar> / x * indicator {0<..<t} x)" by (simp add: field_simps)
+  finally have 
+    2: "(\<lambda>x. LBINT y. \<bar>sin x\<bar> * exp (- (y * x)) * indicator {0<..} y * indicator {0<..<t} x) =
+        (\<lambda>x. \<bar>sin x\<bar> / x * indicator {0<..<t} x)" .
+  { 
+    fix t
+    have *: "AE x in lborel. \<bar>sin x\<bar> / x * indicator {0<..<t} x = abs (sinc x) * indicator {0..t} x"
+      apply (rule AE_I [where N = "{0, t}"])
+      apply (auto split: split_indicator)
+      by (metis lmeasure_eq_0 negligible_insert negligible_sing)
+    have "set_integrable lborel {0<..<t} (\<lambda>x. \<bar>sin x\<bar> / x)"
+      apply (subst integrable_cong_AE [OF _ _ *])
+      apply measurable
+      apply (auto intro!: borel_measurable_continuous_on1 continuous_on_sin continuous_on_id) [3]
+      apply measurable
+      apply (auto intro!: borel_measurable_continuous_on1 continuous_on_sin continuous_on_id)
+      apply (rule set_integrable_abs)
+      apply (rule borel_integrable_atLeastAtMost)
+      by (auto intro: isCont_sinc)
+  } note 3 = this
+  have "AE x \<in> {0..} in lborel. LBINT u=0..\<infinity>. exp (-(u * x)) = 1/x"
+    apply (rule AE_I[where N = "{0}"], auto)
+    using integral_expneg_alpha_atLeast0 using less_eq_real_def by metis
+  hence "Si t = LBINT x=0..t. sin x * (LBINT u=0..\<infinity>. exp (-(u * x)))" unfolding Si_def
+    apply (subst field_divide_inverse)
+    apply (subst inverse_eq_divide)
+    apply (rule interval_integral_cong_AE)
+    apply (rule AE_I' [where N = "{0}"], auto)
+    apply (subst (asm) integral_expneg_alpha_atLeast0) back
+    unfolding einterval_def apply auto
+    apply (subst (asm) min_absorb1)
+    using `t \<ge> 0` by auto
+  also have "\<dots> =  LBINT x. (sin x * indicator {0<..<t} x) * (LBINT u=0..\<infinity>. exp (-(u * x)))"
+    apply (subst interval_lebesgue_integral_def)
+    apply (subst einterval_def)
+    using `t \<ge> 0` by (auto simp add: field_simps greaterThanLessThan_def greaterThan_def
+      lessThan_def Collect_conj_eq)
+  also have "\<dots> = (LBINT x. (LBINT u. sin (fst (x, u)) * exp (-(snd (x, u) * fst (x,u))) * 
+      indicator {0<..} (snd (x, u)) * indicator {0<..<t} (fst (x, u))))"
+    apply (rule integral_cong)
+    apply (case_tac "x \<le> 0", auto)
+    apply (subst interval_lebesgue_integral_cmult (2) [symmetric])
+    apply (simp add: interval_lebesgue_integrable_def zero_ereal_def)
+    apply (rule integral_expneg_alpha_atLeast0, auto)
+    using `t \<ge> 0` unfolding interval_lebesgue_integral_def einterval_def apply auto
+    apply (rule integral_cong)
+    by (simp add: field_simps greaterThan_def)
+  also have "\<dots> = (LBINT u. (LBINT x. sin (fst (x, u)) * exp (-(snd (x, u) * fst (x,u))) * 
+      indicator {0<..} (snd (x, u)) * indicator {0<..<t} (fst (x, u))))"
+    apply (rule P.Fubini_integral [symmetric])
+    apply (subst integrable_abs_iff [symmetric])
+    apply measurable  (* this should be automatic *)
+    apply (rule measurable_fst'', auto intro!: borel_measurable_continuous_on1 
+        continuous_on_sin continuous_on_id)
+    apply (rule P.Fubini_integrable_nonneg)
+    apply measurable
+    apply (rule measurable_fst'', auto intro!: borel_measurable_continuous_on1 
+        continuous_on_sin continuous_on_id)
+    apply (simp_all add: abs_mult)
+    apply (subst 2, rule 3)
+    apply (rule AE_I2)
+    by (rule 1)
+  also have "\<dots> = (LBINT u. (LBINT x. sin x * exp (-u * x) * 
+      indicator {0<..} u * indicator {0<..<t} x))" by simp
+  also have "... = LBINT u=0..\<infinity>. (LBINT x=0..t. sin x * exp (-(u * x)))"
+    using `t >= 0` apply (auto simp add: interval_lebesgue_integral_def zero_ereal_def)
+    by (rule integral_cong, auto split: split_indicator)
+  also have "\<dots> = LBINT u=0..\<infinity>. 1 / (1 + u\<^sup>2) - 1 / (1 + u\<^sup>2) * 
+      (exp (- (u * t)) * (u * sin t + cos t))"
+    apply (subst mult_commute)
+    apply (subst ex_18_4_1 [OF `t >= 0`])
+    apply (rule interval_integral_cong, clarify)
+    (* simp add: field_simps *)
+    by (subst right_diff_distrib, simp)
+  also have "... = (LBINT u=0..\<infinity>. 1 / (1 + u^2)) - (LBINT u=0..\<infinity>. 1 / (1 + u^2) *
+      (exp (- (u * t)) * (u * sin t + cos t)))"
+    apply (rule interval_lebesgue_integral_diff)
+    using  Billingsley_ex_17_5' (1) apply (simp add: zero_ereal_def 
+      interval_lebesgue_integrable_def inverse_eq_divide)
+      apply simp
+      by (rule Si_at_top_lemma (1) [OF `0 \<le> t`])
+  finally have "Si t = pi / 2 - (LBINT u=0..\<infinity>. 1 / (1 + u^2) * exp (-(u * t)) *
+    (u * sin t + cos t))"
+    apply (subst (asm) inverse_eq_divide [symmetric])
+    apply (subst (asm) Billingsley_ex_17_5')
+    by simp
+} note 5 = this
+  have 6: "eventually (\<lambda>t. pi / 2 - (LBINT u=0..\<infinity>. 1 / (1 + u^2) * exp (-(u * t)) *
+    (u * sin t + cos t)) = Si t) at_top"
+    apply (rule eventually_mp [OF _ eventually_ge_at_top [of 0]])
+    apply (rule always_eventually, clarify, rule sym)
+    by (erule 5)
+  show ?thesis
+    apply (rule Lim_transform_eventually [OF 6])
+    apply (subgoal_tac "pi / 2 = pi / 2 - 0")
+    apply (erule ssubst) back
+    apply (rule tendsto_diff, auto)
+    by (rule Si_at_top_lemma)
+qed
+
+lemma iSi_integrable: "interval_lebesgue_integrable lborel (ereal 0)
+     (ereal T) (\<lambda>t. sin (t * \<theta>) / t)"
+proof -
+  have "interval_lebesgue_integrable lborel (ereal 0) (ereal T) (\<lambda>t. \<theta> * sinc (t * \<theta>))"
+    apply (rule interval_lebesgue_integral_cmult)
+    apply (rule interval_integrable_isCont)
+    by (rule continuous_within_compose3 [OF isCont_sinc], auto)
+  (* this shouldn't be so hard! *)
+  thus ?thesis
+    apply (subst interval_lebesgue_integrable_cong_AE)
+    prefer 4 apply assumption
+    prefer 2 
+    apply (subst measurable_lborel1)
+    apply (rule borel_measurable_continuous_on1)
+    apply (rule continuous_at_imp_continuous_on)
+    apply clarify
+    apply (rule continuous_mult_left)
+    apply (rule continuous_within_compose3 [OF isCont_sinc], auto)
+
+    apply measurable apply auto
+    apply (rule borel_measurable_continuous_on1)
+    apply (rule continuous_at_imp_continuous_on)
+    apply auto
+    by (rule AE_I' [where N = "{0}"], auto)
+qed
 
 lemma Billingsley_26_15:
+  fixes \<theta> :: real
   assumes "T \<ge> 0"
-  shows "\<And>\<theta>. LBINT t=ereal 0..T. sin (t * \<theta>) / t = sgn \<theta> * Si (T * \<bar>\<theta>\<bar>)"
-  sorry
+  shows "LBINT t=ereal 0..T. sin (t * \<theta>) / t = sgn \<theta> * Si (T * \<bar>\<theta>\<bar>)"
+proof -
+  {
+    assume "0 < \<theta>"
+    have "(LBINT t=ereal 0..T. sin (t * \<theta>) / t) = (LBINT t=ereal 0..T. sinc (t * \<theta>) * \<theta>)"
+      apply (rule interval_integral_cong_AE)
+      apply (rule AE_I' [where N = "{0}"])
+      by auto
+    also have "\<dots> = (LBINT t=ereal (0 * \<theta>)..T * \<theta>. sinc t)"
+      apply (rule interval_integral_substitution_finite [OF assms])
+      apply (subst mult_commute, rule DERIV_subset)
+      by (auto intro!: derivative_intros continuous_at_imp_continuous_on isCont_sinc)
+    also have "\<dots> = (LBINT t=ereal (0 * \<theta>)..T * \<theta>. sin t / t)"
+      apply (rule interval_integral_cong_AE)
+      apply (rule AE_I' [where N = "{0}"])
+      by auto
+    finally have "(LBINT t=ereal 0..T. sin (t * \<theta>) / t) = (LBINT t=ereal 0..T * \<theta>. sin t / t)"
+      by simp
+    hence "LBINT x. sin (x * \<theta>) * indicator {0<..<T} x / x =
+        LBINT x. sin x * indicator {0<..<T * \<theta>} x / x"
+      using assms `0 < \<theta>` unfolding interval_lebesgue_integral_def einterval_eq zero_ereal_def 
+        by auto
+  } note aux1 = this
+  {
+    assume "0 > \<theta>"
+    have [simp]: "integrable lborel (\<lambda>x. sin (x * \<theta>) * indicator {0<..<T} x / x)"
+      using iSi_integrable [of T \<theta>] assms 
+      by (simp add: interval_lebesgue_integrable_def)
+    have "(LBINT t=ereal 0..T. sin (t * -\<theta>) / t) = (LBINT t=ereal 0..T. sinc (t * -\<theta>) * -\<theta>)"
+      apply (rule interval_integral_cong_AE)
+      apply (rule AE_I' [where N = "{0}"])
+      by auto
+    also have "\<dots> = (LBINT t=ereal (0 * -\<theta>)..T * -\<theta>. sinc t)"
+      apply (rule interval_integral_substitution_finite [OF assms])
+      apply (subst mult_commute, rule DERIV_subset)
+      by (auto intro!: derivative_intros continuous_at_imp_continuous_on isCont_sinc)
+    also have "\<dots> = (LBINT t=ereal (0 * -\<theta>)..T * -\<theta>. sin t / t)"
+      apply (rule interval_integral_cong_AE)
+      apply (rule AE_I' [where N = "{0}"])
+      by auto
+    finally have "(LBINT t=ereal 0..T. sin (t * -\<theta>) / t) = (LBINT t=ereal 0..T * -\<theta>. sin t / t)"
+      by simp
+    hence "LBINT x. sin (x * \<theta>) * indicator {0<..<T} x / x =
+       - (LBINT x. sin x * indicator {0<..<- (T * \<theta>)} x / x)"
+      using assms `0 > \<theta>` unfolding interval_lebesgue_integral_def einterval_eq zero_ereal_def
+        apply (auto simp add: field_simps)
+        apply (case_tac "T = 0", auto)
+        apply (subgoal_tac "T * \<theta> < 0")
+        apply auto
+        by (rule mult_pos_neg, auto)
+  } note aux2 = this
+  show ?thesis
+    using assms unfolding Si_def interval_lebesgue_integral_def sgn_real_def 
+      einterval_eq zero_ereal_def apply auto
+    apply (erule aux1)
+    by (rule aux2, auto)
+qed
+
+lemma sinc_neg [simp]: "sinc (- x) = sinc x" by auto
+
+lemma Si_neg: 
+  fixes T :: real
+  assumes "T \<ge> 0"
+  shows "Si (- T) = - Si T"
+proof -
+  have "LBINT x=ereal 0..T. sinc (- x) * -1 = LBINT y= ereal (- 0)..ereal (- T). sinc y"
+    apply (rule interval_integral_substitution_finite [OF assms])
+    by (auto intro: derivative_intros continuous_at_imp_continuous_on isCont_sinc)
+  also have "(LBINT x=ereal 0..T. sinc (- x) * -1) = -(LBINT x=ereal 0..T. sinc x)"
+    apply (subst sinc_neg, simp)
+    by (rule interval_lebesgue_integral_uminus)
+  finally have *: "-(LBINT x=ereal 0..T. sinc x) = LBINT y= ereal 0..ereal (- T). sinc y"
+    by simp
+  show ?thesis
+    using assms unfolding Si_alt_def
+     apply (subst zero_ereal_def)+
+     by (auto simp add: * [symmetric])
+qed
+
+(* TODO: need a better version of FTC2 *)
+
+lemma has_field_derivative_within_open: "a \<in> s \<Longrightarrow> open s \<Longrightarrow>
+    (f has_field_derivative f') (at a within s) = (f has_field_derivative f') (at a)"
+  unfolding has_field_derivative_def by (rule has_derivative_within_open)
+
+lemma iSi_isCont: "isCont Si x"
+proof -
+  have "Si = (\<lambda>t. LBINT x=ereal 0..ereal t. sinc x)"
+    apply (rule ext, simp add: Si_def zero_ereal_def)
+    apply (rule interval_integral_cong_AE)
+    by (rule AE_I' [where N = "{0}"], auto)
+  thus ?thesis
+    apply (elim ssubst)
+    apply (rule DERIV_isCont)
+    apply (subst has_field_derivative_within_open [symmetric, 
+      where s = "{(min (x - 1) (- 1))<..<(max 1 (x+1))}"], auto)
+    apply (rule DERIV_subset [where s = "{(min (x - 2) (- 2))..(max 2 (x+2))}"])
+    apply (rule interval_integral_FTC2)
+    by (auto intro: continuous_at_imp_continuous_on isCont_sinc)
+qed
+
+lemma borel_measurable_iSi: "f \<in> borel_measurable M \<Longrightarrow> 
+  (\<lambda>x. Si (f x)) \<in> borel_measurable M"
+  apply (rule borel_measurable_continuous_on) back
+  by (rule continuous_at_imp_continuous_on, auto intro: iSi_isCont)
+
+lemma iSi_bounded: "\<exists>B. \<forall>T. abs (Si T) \<le> B"
+proof -
+  from Si_at_top have "eventually (\<lambda>T. dist (Si T) (pi / 2) < 1) at_top"
+    by (elim tendstoD, simp)
+  hence "\<exists>T. \<forall>t \<ge> T. dist (Si t) (pi / 2) < 1" 
+    by (simp add: eventually_at_top_linorder)
+  then obtain T where T [rule_format]: "\<forall>t \<ge> T. dist (Si t) (pi / 2) < 1" ..
+  let ?T' = "max T 0"
+  {
+    fix t
+    assume "t \<ge> ?T'"
+    hence *: "t \<ge> T" by auto
+    from T [OF *]
+    have **: "abs (Si t - pi / 2) < 1" by (simp add: dist_real_def)
+    have "abs (Si t) = abs ((Si t - pi / 2) + pi / 2)" by simp
+    also have "\<dots> \<le> abs (Si t - pi / 2) + abs (pi / 2)" by (rule abs_triangle_ineq)
+    also have "\<dots> \<le> 1 + abs (pi / 2)"
+      by (rule add_right_mono, rule less_imp_le, rule **)
+    finally have "abs (Si t) \<le> 1 + abs (pi / 2)" .
+  } note aux1 = this
+  {
+    fix t 
+    assume *: "t \<le> -?T'"
+    have "abs (Si t) = abs (Si (- (-t)))" by simp
+    also have "\<dots> = abs (Si (- t))"
+      apply (subst Si_neg)
+      using * by auto
+    also have "\<dots> \<le> 1 + abs (pi / 2)"
+      apply (rule aux1)
+      using * by auto
+    finally have "abs (Si t) \<le> 1 + abs (pi / 2)" .
+  } note aux2 = this
+  have "\<exists>M. \<forall>t. -?T' \<le> t \<and> t \<le> ?T' \<longrightarrow> abs (Si t) \<le> M"
+    apply (rule isCont_bounded)
+    by (auto intro!: iSi_isCont continuous_intros)
+  then obtain M where M [rule_format]: "\<forall>t. -?T' \<le> t \<and> t \<le> ?T' \<longrightarrow> abs (Si t) \<le> M" ..
+  let ?B = "max M (1 + abs (pi / 2))"
+  have "\<forall>t. abs (Si t) \<le> ?B"
+  proof
+    fix t
+    show "abs (Si t) \<le> ?B"
+      apply (case_tac "t \<ge> ?T'")
+      apply (rule order_trans)
+      apply (erule aux1, force)
+      apply (case_tac "t \<le> -?T'")
+      apply (rule order_trans)
+      apply (erule aux2, force)
+      apply (rule order_trans)
+      by (rule M, auto)
+  qed
+  thus ?thesis ..
+qed    
 
 end
